WIP: wtraced new causal

nondeterministic_dataflow/Wtraced_Composition.thy
@@ -4,6 +4,244 @@ imports
   "BNA_Operators"
 begin
 
+
+inductive wstep_comp_op where
+  \<open>comp_op wire buf' op1' op2' = comp_op wire buf op1 op2 \<Longrightarrow> wstep_comp_op Tau wire buf buf' op1 op1' op2 op2'\<close>
+| \<open>step Tau op1 op1' \<Longrightarrow> wstep_comp_op Tau wire buf buf' op1' op1'' op2 op2' \<Longrightarrow> wstep_comp_op Tau wire buf buf' op1 op1'' op2 op2'\<close>
+| \<open>step Tau op2 op2' \<Longrightarrow> wstep_comp_op Tau wire buf buf' op1 op1' op2' op2'' \<Longrightarrow> wstep_comp_op Tau wire buf buf' op1 op1' op2 op2''\<close>
+| \<open>wstep_comp_op Tau wire buf buf' op1 op1' op2 op2' \<Longrightarrow> step (Inp p x) op1' op1'' \<Longrightarrow> wstep_comp_op Tau wire buf' buf'' op1'' op1''' op2' op2'' \<Longrightarrow> wstep_comp_op (Inp (Inl p) x) wire buf buf'' op1 op1''' op2 op2''\<close>
+| \<open>wstep_comp_op Tau wire buf buf' op1 op1' op2 op2' \<Longrightarrow> step (Out p x) op2' op2'' \<Longrightarrow> wstep_comp_op Tau wire buf' buf'' op1' op1'' op2'' op2''' \<Longrightarrow> wstep_comp_op (Out (Inr p) x) wire buf buf'' op1 op1'' op2 op2'''\<close>
+| \<open>wstep_comp_op Tau wire buf buf' op1 op1' op2 op2' \<Longrightarrow> step (Out p x) op1' op1'' \<Longrightarrow> wire p = None \<Longrightarrow> wstep_comp_op Tau wire buf' buf'' op1'' op1''' op2' op2'' \<Longrightarrow> wstep_comp_op (Out (Inl p) x) wire buf buf'' op1 op1''' op2 op2''\<close>
+| \<open>wstep_comp_op Tau wire buf buf' op1 op1' op2 op2' \<Longrightarrow> step (Inp p x) op2' op2'' \<Longrightarrow> p \<notin> ran wire \<Longrightarrow> wstep_comp_op Tau wire buf' buf'' op1' op1'' op2'' op2''' \<Longrightarrow> wstep_comp_op (Inp (Inr p) x) wire buf buf'' op1 op1'' op2 op2'''\<close>
+| \<open>step (Out p x) op1 op1' \<Longrightarrow> wire p = Some q \<Longrightarrow> wstep_comp_op Tau wire (BENQ q x buf) buf'' op1' op1'' op2 op2' \<Longrightarrow> wstep_comp_op Tau wire buf buf'' op1 op1'' op2 op2'\<close>
+| \<open>step (Inp p x) op2 op2' \<Longrightarrow> p \<in> ran wire \<Longrightarrow> buf p \<noteq> [] \<Longrightarrow> BHD p buf = x \<Longrightarrow> wstep_comp_op Tau wire (BTL p buf) buf'' op1 op1' op2' op2'' \<Longrightarrow> wstep_comp_op Tau wire buf buf'' op1 op1' op2 op2''\<close>
+
+lemma step_Taus_comp_op:
+  \<open>(step Tau)\<^sup>*\<^sup>* (comp_op wire buf op1 op2) (comp_op wire buf' op1' op2') \<Longrightarrow> wstep_comp_op Tau wire buf buf' op1 op1' op2 op2'\<close>
+  apply (induct "comp_op wire buf op1 op2" arbitrary: buf op1 op2 rule: converse_rtranclp_induct)
+   apply (auto intro: wstep_comp_op.intros elim!: step_comp_op_elim)
+  done
+
+lemma wstep_comp_op:
+  \<open>wstep io (comp_op wire buf op1 op2) (comp_op wire buf' op1' op2') \<longleftrightarrow> wstep_comp_op io wire buf buf' op1 op1' op2 op2'\<close>
+  apply (rule iffI)
+  subgoal
+    unfolding wstep_def
+    apply (erule relcomppE)
+    subgoal for op
+      apply (induct "comp_op wire buf op1 op2" arbitrary: buf op1 op2  rule: converse_rtranclp_induct)
+      subgoal 
+        apply (cases io; simp)
+        subgoal for p x
+          apply (cases p)
+          subgoal
+            apply hypsubst_thin
+            apply (erule relcomppE)
+            apply (auto intro: step_Taus_comp_op wstep_comp_op.intros elim!: step_comp_op_elim)
+            done
+          subgoal
+            apply hypsubst_thin
+            apply (erule relcomppE)
+            apply (auto intro: step_Taus_comp_op wstep_comp_op.intros elim!: step_comp_op_elim)
+            done
+          done
+        subgoal
+          apply hypsubst_thin
+          apply (erule relcomppE)
+          apply (auto intro: step_Taus_comp_op wstep_comp_op.intros elim!: step_comp_op_elim)
+          done
+        subgoal
+          apply hypsubst_thin
+          apply (smt (verit, best) converse_rtranclp_into_rtranclp pick_middlep step_Taus_comp_op)
+          done
+        done
+      subgoal for op buf op1 op2
+        apply (cases io; simp)
+        subgoal for p x
+          apply (cases p)
+          subgoal for p
+            apply hypsubst_thin
+            apply (erule relcomppE)
+            subgoal for op''
+              apply (auto intro: step_Taus_comp_op wstep_comp_op.intros elim!: step_comp_op_elim)
+                 apply hypsubst_thin
+              subgoal
+                apply (drule meta_spec)+
+                apply (drule meta_mp)
+                 apply (rule refl)
+                apply (erule wstep_comp_op.cases)
+                        apply (auto intro: step_Taus_comp_op wstep_comp_op.intros elim!: step_comp_op_elim)
+                done
+              subgoal
+                apply (drule meta_spec)+
+                apply (drule meta_mp)
+                 apply (rule refl)
+                apply (erule wstep_comp_op.cases)
+                        apply (auto intro: step_Taus_comp_op wstep_comp_op.intros elim!: step_comp_op_elim)
+                done
+              subgoal
+                apply (drule meta_spec)+
+                apply (drule meta_mp)
+                 apply (rule refl)
+                apply (erule wstep_comp_op.cases)
+                        apply (auto intro: step_Taus_comp_op wstep_comp_op.intros elim!: step_comp_op_elim)
+                done
+              subgoal
+                apply (drule meta_spec)+
+                apply (drule meta_mp)
+                 apply (rule refl)
+                apply (erule wstep_comp_op.cases)
+                        apply (auto intro: step_Taus_comp_op wstep_comp_op.intros elim!: step_comp_op_elim)
+                done
+              done
+            done
+          subgoal for p
+            apply hypsubst_thin
+            apply (erule relcomppE)
+            subgoal for op''
+              apply (auto intro: step_Taus_comp_op wstep_comp_op.intros elim!: step_comp_op_elim)
+                 apply hypsubst_thin
+              subgoal
+                apply (drule meta_spec)+
+                apply (drule meta_mp)
+                 apply (rule refl)
+                apply (erule wstep_comp_op.cases)
+                        apply (auto intro: step_Taus_comp_op wstep_comp_op.intros elim!: step_comp_op_elim)
+                done
+              subgoal
+                apply (drule meta_spec)+
+                apply (drule meta_mp)
+                 apply (rule refl)
+                apply (erule wstep_comp_op.cases)
+                        apply (auto intro: step_Taus_comp_op wstep_comp_op.intros elim!: step_comp_op_elim)
+                done
+              subgoal
+                apply (drule meta_spec)+
+                apply (drule meta_mp)
+                 apply (rule refl)
+                apply (erule wstep_comp_op.cases)
+                        apply (auto intro: step_Taus_comp_op wstep_comp_op.intros elim!: step_comp_op_elim)
+                done
+              subgoal
+                apply (drule meta_spec)+
+                apply (drule meta_mp)
+                 apply (rule refl)
+                apply (erule wstep_comp_op.cases)
+                        apply (auto intro: step_Taus_comp_op wstep_comp_op.intros elim!: step_comp_op_elim)
+                done
+              done
+            done
+          done
+        subgoal for p x
+          apply (cases p)
+          subgoal for p
+            apply hypsubst_thin
+            apply (erule relcomppE)
+            subgoal for op''
+              apply (auto intro: step_Taus_comp_op wstep_comp_op.intros elim!: step_comp_op_elim)
+                 apply hypsubst_thin
+              subgoal
+                apply (drule meta_spec)+
+                apply (drule meta_mp)
+                 apply (rule refl)
+                apply (erule wstep_comp_op.cases)
+                        apply (auto intro: step_Taus_comp_op wstep_comp_op.intros elim!: step_comp_op_elim)
+                done
+              subgoal
+                apply (drule meta_spec)+
+                apply (drule meta_mp)
+                 apply (rule refl)
+                apply (erule wstep_comp_op.cases)
+                        apply (auto intro: step_Taus_comp_op wstep_comp_op.intros elim!: step_comp_op_elim)
+                done
+              subgoal
+                apply (drule meta_spec)+
+                apply (drule meta_mp)
+                 apply (rule refl)
+                apply (erule wstep_comp_op.cases)
+                        apply (auto intro: step_Taus_comp_op wstep_comp_op.intros elim!: step_comp_op_elim)
+                done
+              subgoal
+                apply (drule meta_spec)+
+                apply (drule meta_mp)
+                 apply (rule refl)
+                apply (erule wstep_comp_op.cases)
+                        apply (auto intro: step_Taus_comp_op wstep_comp_op.intros elim!: step_comp_op_elim)
+                done
+              done
+            done
+          subgoal for p
+            apply hypsubst_thin
+            apply (erule relcomppE)
+            subgoal for op''
+              apply (auto intro: step_Taus_comp_op wstep_comp_op.intros elim!: step_comp_op_elim)
+                 apply hypsubst_thin
+              subgoal
+                apply (drule meta_spec)+
+                apply (drule meta_mp)
+                 apply (rule refl)
+                apply (erule wstep_comp_op.cases)
+                        apply (auto intro: step_Taus_comp_op wstep_comp_op.intros elim!: step_comp_op_elim)
+                done
+              subgoal
+                apply (drule meta_spec)+
+                apply (drule meta_mp)
+                 apply (rule refl)
+                apply (erule wstep_comp_op.cases)
+                        apply (auto intro: step_Taus_comp_op wstep_comp_op.intros elim!: step_comp_op_elim)
+                done
+              subgoal
+                apply (drule meta_spec)+
+                apply (drule meta_mp)
+                 apply (rule refl)
+                apply (erule wstep_comp_op.cases)
+                        apply (auto intro: step_Taus_comp_op wstep_comp_op.intros elim!: step_comp_op_elim)
+                done
+              subgoal
+                apply (drule meta_spec)+
+                apply (drule meta_mp)
+                 apply (rule refl)
+                apply (erule wstep_comp_op.cases)
+                        apply (auto intro: step_Taus_comp_op wstep_comp_op.intros elim!: step_comp_op_elim)
+                done
+              done
+            done
+          done
+        subgoal
+          by (auto intro: step_Taus_comp_op wstep_comp_op.intros elim!: step_comp_op_elim)
+        done
+      done
+    done
+  subgoal
+    apply (induct pred: wstep_comp_op)
+            apply force
+           apply blast
+          apply blast
+    subgoal for wire buf buf' op1 op1' op2 op2' p x op1'' buf'' op1''' op2''
+      apply simp
+      apply (smt (verit, ccfv_threshold) estep.simps(2) relcompp_apply step_comp_op_L_Inp wstep_def)
+      done
+    subgoal for wire buf buf' op1 op1' op2 op2' p x op2'' buf'' op1'' op2'''
+      apply simp
+      apply (smt (verit, best) estep.simps(3) relcomppI step_comp_op_R_Out wstep_def)
+      done
+    subgoal
+      apply simp
+      apply (smt (verit, ccfv_threshold) domIff estep.simps(3) relcomppI step_comp_op_L_Out wstep_def)
+      done
+    subgoal
+      apply simp
+      apply (smt (verit, best) estep.simps(2) relcompp_apply step_comp_op_R_Inp wstep_def)
+      done
+    subgoal
+      apply simp
+      apply (meson converse_rtranclp_into_rtranclp step_Tau_comp_op_L_alt)
+      done
+    subgoal
+      by blast
+    done
+  done
+
 inductive visible_cause for wire where
   "visible_cause wire buf (LCons (VInp (Inl p) x) ios) (LCons (VInp p x) ios1) ios2 buf ios ios1 ios2"
 | "visible_cause wire buf (LCons (VOut (Inr p) x) ios) ios1 (LCons (VOut p x) ios2) buf ios ios1 ios2"
@@ -16,43 +254,8 @@ inductive visible_cause for wire where
    visible_cause wire buf ios ios1 (LCons (VInp p x) ios2) buf' ios ios1' ios2'"
 
 coinductive causal for wire where
- "causal wire buf' ios' ios1' ios2' \<Longrightarrow> visible_cause wire buf ios ios1 ios2 buf' ios' ios1' ios2' \<Longrightarrow> causal wire buf ios ios1 ios2"
-(* | "causal wire buf ios1 ios2 \<Longrightarrow> wire p = None \<Longrightarrow> causal wire buf (LCons (VOut p x) ios1) ios2"
-| "causal wire (BENQ q x buf) ios1 ios2 \<Longrightarrow> wire p = Some q \<Longrightarrow> causal wire buf (LCons (VOut p x) ios1) ios2"
-| "causal wire buf ios1 ios2 \<Longrightarrow> causal wire buf ios1 (LCons (VOut p y) ios2)"
-| "causal wire buf ios1 ios2 \<Longrightarrow> p \<notin> ran wire \<Longrightarrow> causal wire buf ios1 (LCons (VInp p y) ios2)"
-| "causal wire (BTL p buf) ios1 ios2 \<Longrightarrow> buf p \<noteq> [] \<Longrightarrow> y = BHD p buf \<Longrightarrow> p \<in> ran wire \<Longrightarrow> causal wire buf ios1 (LCons (VInp p y) ios2)" *)
-(* 
-
-abbreviation "VIO_Inls ios \<equiv>
-  lmap (case_VIO (case_sum VInp VInp) (case_sum VOut VOut)) (lfilter (case_VIO (case_sum \<top> \<bottom>) (case_sum \<top> \<bottom>)) ios)"
-
-abbreviation "VIO_Inrs ios \<equiv>
-  lmap (case_VIO (case_sum VInp VInp) (case_sum VOut VOut)) (lfilter (case_VIO (case_sum \<bottom> \<top>) (case_sum \<bottom> \<top>)) ios)"
-
-abbreviation visible_VIO where "visible_VIO wire io \<equiv> case_VIO (\<lambda>p _. case_sum (\<lambda> _. True) (\<lambda> q. q \<notin> ran wire) p) (\<lambda> p _. case_sum (\<lambda> q. q \<notin> dom wire) (\<lambda> _. True) p) io" 
-
-lemma causal_LCons_VInp_Inl:
-  "causal wire buf (LCons (VInp p x) ios1) ios2 \<Longrightarrow>
-   causal wire buf ios1 ios2"
-  apply (coinduction arbitrary: buf ios1 ios2 rule: causal.coinduct)
-  subgoal for buf ios1 ios2
-    apply (erule causal.cases)
-          apply simp_all
-    apply hypsubst_thin
-    apply (smt (verit) causal.cases)
-    done
-  done
-
-lemma causal_LCons_VOut_Inr:
-  "causal wire buf ios (LCons (VOut p x) ios2) \<Longrightarrow>
-   causal wire buf ios1 ios2"
-  apply (coinduction arbitrary: buf ios1 ios2 rule: causal.coinduct)
-  subgoal for buf ios1 ios2
-    apply (erule causal.cases)
-          apply simp_all
-    apply hypsubst_thin
-    oops *)
+  "causal wire buf LNil LNil LNil"
+| "causal wire buf' ios' ios1' ios2' \<Longrightarrow> ios \<noteq> LNil \<Longrightarrow> visible_cause wire buf ios ios1 ios2 buf' ios' ios1' ios2' \<Longrightarrow> causal wire buf ios ios1 ios2"
 
 lemma visible_cause_VInp_Inl_LNil_False:
   "visible_cause wire buf (LCons (VInp (Inl lp) x) ios) ios1 ios2 buf' ios' ios1' ios2' \<Longrightarrow>
@@ -62,67 +265,91 @@ lemma visible_cause_VInp_Inl_LNil_False:
     apply auto
   done
 
-lemma visible_cause_VInp_Inr:
+lemma visible_cause_wtraced_wstep:
   "visible_cause wire buf IOS ios1 ios2 buf' ios' ios1' ios2' \<Longrightarrow>
-   IOS = LCons (VInp (Inr p) x) ios \<Longrightarrow>
+   IOS = (LCons X ios) \<Longrightarrow>
    wtraced op1 ios1 \<Longrightarrow>
    wtraced op2 ios2 \<Longrightarrow>
-   \<exists> op1' op2'. wstep (Inp (Inr p) x) (comp_op wire buf op1 op2) (comp_op wire buf' op1' op2') \<and> wtraced op1' ios1' \<and> wtraced op2' ios2' \<and> ios' = ios"
+   \<exists> op1' op2'. wstep (io_of_vio X) (comp_op wire buf op1 op2) (comp_op wire buf' op1' op2') \<and> wtraced op1' ios1' \<and> wtraced op2' ios2' \<and> ios' = ios"
   apply (induct buf IOS ios1 ios2 buf' ios' ios1' ios2' arbitrary: op1 op2 pred: visible_cause)
-       apply auto
-  subgoal for buf ios1 ios2 op1 op2
+       apply simp_all
+  subgoal
+    apply (erule wtraced.cases)
+     apply simp_all
+    subgoal for vio op op'
+      apply (cases vio; simp)
+      using wstep_comp_op_L_Inp apply fastforce
+      done
+    done
+  subgoal
     apply (rotate_tac 2)
     apply (erule wtraced.cases)
      apply simp_all
     subgoal for vio op op'
       apply (cases vio; simp)
-      using wstep_comp_op_R_Inp apply fastforce
+      apply (metis io_of_vio.simps(2) wstep_comp_op_R_Out)
       done
     done
-  subgoal for q xa buf ios1 ios2 buf' ios1' ios2' pa op1 op2
+  subgoal
+    apply (erule wtraced.cases)
+     apply simp_all
+    subgoal for vio op op'
+      apply (cases vio; simp)
+      apply (metis domIff io_of_vio.simps(2) wstep_comp_op_L_Out)
+      done
+    done
+  subgoal for p buf x ios1 ios2 op1 op2
     apply (rotate_tac 3)
     apply (erule wtraced.cases)
      apply simp_all
     subgoal for vio op op'
       apply (cases vio; simp)
-      apply (drule meta_spec)+
-      apply (drule meta_mp)
-      apply assumption
-      apply (drule meta_mp)
-      apply assumption
-      apply safe
-      subgoal for p op1' op2'
-        apply (rule exI[of _ op1'])
-        apply (rule exI[of _ op2'])
-        apply simp
-        apply hypsubst_thin
-        apply (subgoal_tac "(step Tau)\<^sup>*\<^sup>* (comp_op wire buf op op2) (comp_op wire (BENQ q xa buf) op' op2)")
-         defer
-        subgoal
-          by (metis wstep_Tau_comp_op_L wstep_steps_Tau)
-        apply (smt (verit) relcompp_apply rtranclp_trans wstep_def)
-        done
+      apply (metis io_of_vio.simps(1) wstep_comp_op_R_Inp)
       done
     done
-  subgoal for pa buf ios1 ios2 buf' ios1' ios2' op1 op2
-   apply (rotate_tac 5)
+  subgoal for q x buf iosa ios1 ios2 buf' ios1' ios2' p op1 op2
     apply (erule wtraced.cases)
      apply simp_all
     subgoal for vio op op'
       apply (cases vio; simp)
       apply (drule meta_spec)+
       apply (drule meta_mp)
-      apply assumption
+       apply assumption
       apply (drule meta_mp)
-      apply assumption
+       apply assumption
       apply safe
       subgoal for p op1' op2'
         apply (rule exI[of _ op1'])
         apply (rule exI[of _ op2'])
         apply simp
         apply hypsubst_thin
-        apply (subgoal_tac "(step Tau)\<^sup>*\<^sup>* (comp_op wire buf op1 op) (comp_op wire (BTL pa buf) op1 op')")
-        defer
+        apply (subgoal_tac "(step Tau)\<^sup>*\<^sup>* (comp_op wire buf op op2) (comp_op wire (BENQ q x buf) op' op2)")
+         defer
+        subgoal
+          by (metis wstep_Tau_comp_op_L wstep_steps_Tau)
+        apply (smt (verit, ccfv_threshold) relcompp_apply rtranclp_trans wstep_def)
+        done
+      done
+    done
+  subgoal for p buf iosa ios1 ios2 buf' ios1' ios2' x op1 op2
+    apply (rotate_tac 7)
+    apply (erule wtraced.cases)
+     apply simp_all
+    subgoal for vio op op'
+      apply (cases vio; simp)
+      apply (drule meta_spec)+
+      apply (drule meta_mp)
+       apply assumption
+      apply (drule meta_mp)
+       apply assumption
+      apply safe
+      subgoal for p' op1' op2'
+        apply (rule exI[of _ op1'])
+        apply (rule exI[of _ op2'])
+        apply simp
+        apply hypsubst_thin
+        apply (subgoal_tac "(step Tau)\<^sup>*\<^sup>* (comp_op wire buf op1 op) (comp_op wire (BTL p buf) op1 op')")
+         defer
         subgoal
           by (metis wstep_Tau_comp_op_R wstep_steps_Tau)
         apply (smt (verit) relcompp_apply rtranclp_trans wstep_def)
@@ -131,11 +358,49 @@ lemma visible_cause_VInp_Inr:
     done
   done
 
+lemma wstep_comp_op_wfinished_preserve:
+  "wstep io (comp_op wire buf op1 op2) op \<Longrightarrow>
+   wfinished op1 \<Longrightarrow>
+   wfinished op2 \<Longrightarrow>
+   io \<noteq> Tau \<Longrightarrow>
+   False"
+  unfolding wstep_def
+  apply (erule relcomppE)
+  subgoal for op'
+    apply (rotate_tac 3)
+    apply (induct "comp_op wire buf op1 op2" arbitrary: buf op1 op2  rule: converse_rtranclp_induct)
+    subgoal for buf op1 op2
+      apply (cases io; simp; hypsubst_thin?)
+      subgoal for p x
+        apply (erule relcomppE)
+        apply (elim step_comp_op_elim)
+               apply auto
+         apply (metis io_of_vio.simps(1) step_not_wfinished)+
+        done
+      subgoal for p x
+        apply (erule relcomppE)
+        apply (elim step_comp_op_elim)
+               apply auto
+         apply (metis io_of_vio.simps(2) step_not_wfinished)+
+        done
+      done
+    subgoal for op' buf' op1' op2'
+      apply simp
+      apply (elim step_comp_op_elim)
+             apply (auto dest: step_Tau_wfinished)
+      subgoal
+        by (metis io_of_vio.simps(2) step_not_wfinished)
+
+      by (metis io_of_vio.simps(1) step_not_wfinished)
+    done
+  done
+
 lemma
   "wtraced (comp_op wire buf op1 op2) ios = 
    (\<exists> ios1 ios2. wtraced op1 ios1 \<and> wtraced op2 ios2 \<and> causal wire buf ios ios1 ios2)"
   apply (rule iffI)
   subgoal
+    apply (erule wtraced.cases; simp)
     sorry
   subgoal
     apply (elim exE conjE)
@@ -146,135 +411,43 @@ lemma
         subgoal
           apply (simp add: lfilter_eq_LNil)
           apply hypsubst_thin
-          sorry
+          apply (erule causal.cases)
+           apply simp_all
+          apply hypsubst_thin
+          apply (erule wtraced.cases; simp)
+          apply (erule wtraced.cases; simp)
+          apply hypsubst_thin
+          apply (subst wfinished_no_wstep)
+          apply safe
+          using wstep_comp_op_wfinished_preserve apply (metis io_of_vio_not_Tau(1))
+          done
         subgoal for io ios
           apply (cases io)
           subgoal for p x
-            apply (cases p)
-            subgoal for lp
-              apply (simp split: if_splits)
-              apply hypsubst_thin
-              apply (erule wtraced.cases)
-              subgoal
-                apply (erule causal.cases)
-                apply auto
-                apply hypsubst_thin
-                using visible_cause_VInp_Inl_LNil_False apply fast
-                done
-              subgoal
-                apply hypsubst_thin
-                apply (erule causal.cases)
-                apply auto
-                sorry
-              done
-            subgoal for rp
-              apply (simp split: if_splits)
-              apply hypsubst_thin
-              apply rotate_tac
-              apply (erule wtraced.cases)
-              subgoal sorry
-              subgoal for vio op op' lxs
-                apply hypsubst_thin
-                apply (erule causal.cases)
-                apply auto
-                subgoal for buf' ios' ios1' ios2'
-                  apply (drule visible_cause_VInp_Inr)
-                  apply simp_all
-                    apply (rule wtraced.Step)
-                    apply assumption+
-                  apply safe
-                  apply (intro conjI exI)
-                   apply assumption
-                  apply (intro conjI exI disjI1)
-                     apply (rule refl)
-                    apply assumption+
-                  done
-                done
-              done
+            apply simp
+            apply hypsubst_thin
+            apply (erule causal.cases)
+             apply simp
+            apply hypsubst_thin
+            apply (drule visible_cause_wtraced_wstep)
+               apply simp_all
+            apply force
             done
           subgoal for p x
-            apply (cases p)
-            subgoal for lp
-              apply (simp split: if_splits)
-              apply hypsubst_thin
-              apply (erule wtraced.cases)
-               apply simp_all
-              subgoal
-                apply hypsubst_thin
-                sorry
-              subgoal for vio op op' lx
-                apply hypsubst_thin
-                sorry
-              done
-            subgoal for rp
-              apply (simp split: if_splits)
-              apply hypsubst_thin
-              apply rotate_tac
-              apply (erule wtraced.cases)
-              subgoal sorry
-              subgoal for vio op op' lxs
-                apply hypsubst_thin
-
-end
-                by simp
-              subgoal for vio op op' ios1'
-                apply (simp split: if_splits)
-                subgoal
-                 apply hypsubst_thin
-                  apply (drule causal_LCons_VInp_Inl)
-                    apply (intro exI conjI)
-                     apply (rule wstep_comp_op_L_Inp)
-                       apply assumption
-                      apply (rule refl)+
-                    apply blast
-                  done
-                subgoal
-                 apply hypsubst_thin
-                  apply (simp split: VIO.splits)
-                  subgoal for p x
-                  apply (intro exI conjI)
-                     apply (rule wstep_trans(2)[of _ "comp_op wire (BENQ p x buf) op' op2"])
-                    unfolding wstep_def
-                    subgoal sorry
-              
-
-                    find_theorems wtraced wstep
-
-
-end
-                  apply (rule step_Tau_comp_op_L)
-
-                  find_theorems wstep name: trans
-
-
-
-end
-
-
-                  subgoal for ios2 p y
-                    apply hypsubst_thin
-                    apply (intro exI conjI)
-                     apply (rule wstep_comp_op_L_Inp)
-                       apply assumption
-                      apply (rule refl)+
-                    apply (rule disjI1)
-                    apply (intro exI conjI)
-                      apply (rule refl)+
-                        apply assumption+
-                     apply fastforce
-                    apply (rule causal.intros(5)) 
-                    apply (rule causal_LCons_VInp_Inl)
-                    apply force
-                    done
-                  subgoal for ios2 p y
-                    apply hypsubst_thin
-                    sledgehammer             
-
-                    find_theorems "ldropWhile _ _ = LCons _ _"
-
-        find_theorems lfilter LNil
-
-  oops
+            apply simp
+            apply hypsubst_thin
+            apply (erule causal.cases)
+            apply simp
+            apply hypsubst_thin
+            apply (drule visible_cause_wtraced_wstep)
+            apply simp_all
+            apply force
+            done
+          done
+        done
+      done
+    done
+  done
 
 
 end
